Pos num

src/nat.lean
@@ -2,7 +2,6 @@ import data.num.lemmas
 import lists
 
 namespace pos_num
-#exit
 def to_trailing_bits : pos_num → list bool
 | 1 := []
 | (bit0 xs) := ff :: xs.to_trailing_bits
@@ -21,10 +20,14 @@ def equiv_list_bool : pos_num ≃ list bool :=
   equiv_list_bool (bit0 n) = ff :: equiv_list_bool n := rfl
 @[simp] lemma equiv_list_bool_bit1 (n : pos_num) :
   equiv_list_bool (bit1 n) = tt :: equiv_list_bool n := rfl
+@[simp] lemma equiv_list_bool_symm_nil : equiv_list_bool.symm [] = 1 := rfl
 @[simp] lemma equiv_list_bool_symm_cons_tt (l : list bool) :
   equiv_list_bool.symm (tt :: l) = bit1 (equiv_list_bool.symm l) := rfl
 @[simp] lemma equiv_list_bool_symm_cons_ff (l : list bool) :
   equiv_list_bool.symm (ff :: l) = bit0 (equiv_list_bool.symm l) := rfl
+@[simp] lemma equiv_list_bool_len_zero_iff (n : pos_num) : (equiv_list_bool n).length = 0 ↔ n = 1 :=
+by simp [list.length_eq_zero, equiv.apply_eq_iff_eq_symm_apply]
+
 
 @[simp] lemma succ_inj_iff {x y : pos_num} : x.succ = y.succ ↔ x = y :=
 by { split, { intro h, apply_fun (λ (n : pos_num), (n : ℕ)) at h, simpa using h, }, { rintro rfl, refl, } }
@@ -35,7 +38,7 @@ section
 variables {α β γ : Type*} [polycodable α] [polycodable β] [polycodable γ]
 
 open pos_num
-open polycodable (encode decode)
+open ptree.pencodable (encode decode)
 
 local attribute [instance] unary_nat_encode
 
@@ -53,20 +56,11 @@ lemma polytime_fun.pos_num_equiv_list_bool_sym : polytime_fun equiv_list_bool.sy
 by polyfun
 
 lemma pos_num.succ_list_bool (n : pos_num) :
-  equiv_list_bool n.succ = (equiv_list_bool n).rec' (λ (l : list bool) (ih : list bool), cond l.head (ff :: ih) (tt :: l.tail)) [ff] :=
+  equiv_list_bool n.succ = (equiv_list_bool n).tails.foldr (λ (l : list bool) (ih : list bool), if l.head' = some ff then tt :: l.tail else ff :: ih) [] :=
 begin
   induction n with tl ih tl ih,
   { refl, }, { simp [pos_num.succ, ih], }, { simp [pos_num.succ, ih], }
 end
-
-@[simp] lemma polysize_fun.encode_tt_sizeof : (encode tt).sizeof = 1 :=
-by simp [encode]
-
-@[simp] lemma polysize_fun.encode_ff_sizeof : (encode ff).sizeof = 3 :=
-by simp [encode]
-
-lemma polysize_fun.encode_tail_sizeof_le (l : list α) : (encode l.tail).sizeof ≤ (encode l).sizeof :=
-by { cases l; simp, }
 
 @[polyfun]
 lemma polytime_fun.pos_num_bit0 : polytime_fun pos_num.bit0 :=
@@ -76,47 +70,68 @@ by { convert_to polytime_fun (λ n, equiv_list_bool.symm (ff :: equiv_list_bool 
 lemma polytime_fun.pos_num_bit1 : polytime_fun pos_num.bit1 :=
 by { convert_to polytime_fun (λ n, equiv_list_bool.symm (tt :: equiv_list_bool n)), { ext n, simp, }, polyfun, }
 
-@[simp] lemma encode_pos_num_one : (encode one).sizeof = 1 :=
+@[simp] lemma encode_pos_num_one : (encode (1 : pos_num)).sizeof = 1 :=
 by { simp [polycodable.encode_pos_num], }
 
 @[simp] lemma encode_pos_num_bit0 (n : pos_num) :
-  (encode n.bit0).sizeof = 4 + (encode n).sizeof :=
-by { simp [polycodable.encode_pos_num], }
+  (encode n.bit0).sizeof = (encode n).sizeof + 4 :=
+by { simp [polycodable.encode_pos_num, add_comm], }
 
 @[simp] lemma encode_pos_num_bit1 (n : pos_num) :
-  (encode n.bit1).sizeof = 2 + (encode n).sizeof :=
-by { simp [polycodable.encode_pos_num], }
+  (encode n.bit1).sizeof = (encode n).sizeof + 2 :=
+by { simp [polycodable.encode_pos_num, add_comm], }
+
+lemma polysize_fun_safe.bit0 (α : Type*) [ptree.pencodable α] : polysize_fun_safe (λ (_ : α) (n : pos_num), n.bit0) :=
+⟨4, λ _ _, by simp⟩
+
+lemma polysize_fun_safe.bit1 (α : Type*) [ptree.pencodable α] : polysize_fun_safe (λ (_ : α) (n : pos_num), n.bit1) :=
+⟨2, λ _ _, by simp⟩
 
 @[polyfun]
 lemma polytime_fun.pos_num_succ : polytime_fun pos_num.succ :=
 begin
-  convert_to polytime_fun (λ n, ((equiv_list_bool n).rec'
-    (λ l (ih : pos_num), cond l.head ih.bit0 (equiv_list_bool.symm l.tail).bit1) 2)),
-  { ext n, induction n with _ ih _ ih, { refl, }, all_goals { simp [pos_num.succ, ih], }, },
-  polyfun,
-  use polynomial.monomial 1 1 + 3,
-  intros, cases l.head; simp [polycodable.encode_pos_num]; linarith only [polysize_fun.encode_tail_sizeof_le l],
+  convert_to polytime_fun (λ n : pos_num, equiv_list_bool.symm n.succ.equiv_list_bool), { simp, },
+  simp_rw pos_num.succ_list_bool, polyfun, /- TODO: Fix -/ { apply polytime_fun.comp; polyfun, },
+  apply polysize_fun_safe.ite, { simp, apply polysize_of_polytime_fun, polyfun, }, exact polysize_fun_safe.cons.comp (polysize_uniform_of_fin_range _) polysize_fun_safe.id,
 end
 
-lemma pos_num_add_eq : ∀ (m n : pos_num),
-  (m.add n) = ((equiv_list_bool m).zip (equiv_list_bool n))
-    .foldr (λ bs ih, cond bs.1 
-      (cond bs.2 ih.succ.bit0 ih.bit1)
-      (cond bs.2 ih.bit1 ih.bit0))
-      (if (equiv_list_bool m).length ≤ (equiv_list_bool n).length then 
-        (equiv_list_bool.symm ((equiv_list_bool n).drop (equiv_list_bool m).length)).succ
-       else 
-        (equiv_list_bool.symm ((equiv_list_bool m).drop (equiv_list_bool n).length)).succ)
-| 1 m := by { simp, cases m; simp [pos_num.add], refl, }
-| n 1 := by { simp, cases n; simp [pos_num.add], refl, }
-| (pos_num.bit0 a) (pos_num.bit0 b) := by { simp [pos_num.add], apply pos_num_add_eq, }
-| (pos_num.bit1 a) (pos_num.bit1 b) := by { simp [pos_num.add], apply pos_num_add_eq, }
-| (pos_num.bit1 a) (pos_num.bit0 b) := by { simp [pos_num.add], apply pos_num_add_eq, }
-| (pos_num.bit0 a) (pos_num.bit1 b) := by { simp [pos_num.add], apply pos_num_add_eq, }
+private def add' (m n : pos_num) : pos_num :=
+((equiv_list_bool m).zip (equiv_list_bool n))
+  .foldr (λ bs ih, cond bs.1 
+  (cond bs.2 ih.succ.bit0 ih.bit1)
+  (cond bs.2 ih.bit1 ih.bit0))
+  (if (equiv_list_bool m).length ≤ (equiv_list_bool n).length then 
+    (equiv_list_bool.symm ((equiv_list_bool n).drop (equiv_list_bool m).length)).succ
+    else 
+    (equiv_list_bool.symm ((equiv_list_bool m).drop (equiv_list_bool n).length)).succ)
 
-lemma polytime_fun.pos_num_add : polytime_fun₂ @pos_num.add :=
+@[simp] private lemma add'_case0 (m : pos_num) : add' 1 m = m.succ := by simp [add']
+@[simp] private lemma add'_case1 (n : pos_num) : add' n 1 = n.succ := by simpa [add'] using eq.symm
+@[simp] private lemma add'_case2 (m n : pos_num) : add' m.bit0 n.bit0 = (add' m n).bit0 := by simp [add']
+@[simp] private lemma add'_case3 (m n : pos_num) : add' m.bit1 n.bit1 = (add' m n).succ.bit0 := by simp [add']
+@[simp] private lemma add'_case4 (m n : pos_num) : add' m.bit0 n.bit1 = (add' m n).bit1 := by simp [add']
+@[simp] private lemma add'_case5 (m n : pos_num) : add' m.bit1 n.bit0 = (add' m n).bit1 := by simp [add']
+
+lemma add_eq_add (m n : pos_num) : m.add n = m + n := rfl
+
+lemma pos_num_add_eq : ∀ (m n : pos_num),
+  (m.add n) = add' m n
+| 1 m := by simp [one_add, add_eq_add]
+| n 1 := by simp [add_one, add_eq_add]
+| (pos_num.bit0 a) (pos_num.bit0 b) := by simpa [pos_num.add] using pos_num_add_eq a b
+| (pos_num.bit1 a) (pos_num.bit1 b) := by simpa [pos_num.add] using pos_num_add_eq a b
+| (pos_num.bit1 a) (pos_num.bit0 b) := by simpa [pos_num.add] using pos_num_add_eq a b
+| (pos_num.bit0 a) (pos_num.bit1 b) := by simpa [pos_num.add] using pos_num_add_eq a b
+
+private lemma polytime_fun.pos_num_add' : polytime_fun₂ add' :=
 begin
-  change polytime_fun₂ (λ _ _, _), simp_rw pos_num_add_eq, polyfun,
+  change polytime_fun₂ (λ _ _, _), polyfun,
+end
+
+
+lemma polytime_fun.pos_num_add : polytime_fun₂ pos_num.add :=
+begin
+  change polytime_fun₂ (λ _ _, _), simp_rw pos_num_add_eq, --polyfun,
 end
 
 
